theories/examples/macros.v
@@ -2,7 +2,7 @@ From iris.algebra Require Import frac.
 From iris.proofmode Require Import tactics.
 Require Import Eqdep_dec List.
 From cap_machine Require Import rules logrel macros_helpers map_simpl.
-From cap_machine Require Export iris_extra addr_reg_sample contiguous malloc.
+From cap_machine Require Export iris_extra addr_reg_sample contiguous malloc assert.
 
 Section macros.
   Context {Σ:gFunctors} {memg:memG Σ} {regg:regG Σ}
@@ -153,73 +153,63 @@ Section macros.
   (* ------------------------------------- ASSERT ------------------------------------ *)
   (* --------------------------------------------------------------------------------- *)
 
-  (* The assert macro relies on a convention for the failure flag. This file contains the
-     failure subroutine *)
-
-  (* The convention for the failure flag: one address after the last instruction of the failure subroutine *)
-  (* failing the assert will set the flag to 1 and then crash the program to a Failed configuration. The flag
-     capability is at one address after the instructions *)
-  Definition assert_fail_instrs :=
-    [move_r r_t1 PC;
-    lea_z r_t1 6;
-    load_r r_t1 r_t1;
-    store_z r_t1 1;
-    move_z r_t1 0;
-    halt].
-
-  Definition assert_fail a :=
-    ([∗ list] a_i;w_i ∈ a;(assert_fail_instrs), a_i ↦ₐ w_i)%I.
-
-  (* f_a is the offset of the failure subroutine in the linking table *)
-  (* assert r z asserts that the register r contains the integer z *)
-  (* r is assumed not to be r_t1 *)
-  Definition assert_r_z_instrs f_a r z :=
+  Definition assert_instrs f_a :=
     fetch_instrs f_a ++
-    [sub_r_z r r z;
-    jnz r_t1 r;
-    move_z r_t1 0].
+    [move_r r_t2 r_t0;
+     move_r r_t0 PC;
+     lea_z r_t0 3;
+     jmp r_t1;
+     move_r r_t0 r_t2;
+     move_z r_t1 0;
+     move_z r_t2 0].
 
-  Definition assert_r_z a f_a r z :=
-    ([∗ list] a_i;w_i ∈ a;(assert_r_z_instrs f_a r z), a_i ↦ₐ w_i)%I.
+  Definition assert a f_a :=
+    ([∗ list] a_i;w_i ∈ a;(assert_instrs f_a), a_i ↦ₐ w_i)%I.
 
   (* Spec for assertion success *)
   (* Since we are not jumping to the failure subroutine, we do not need any assumptions
      about the failure subroutine *)
-  Lemma assert_r_z_success a f_a r z pc_p pc_b pc_e a_first a_last
-        b_link e_link a_link a_entry fail_cap w_r φ :
+  Lemma assert_success a f_a pc_p pc_b pc_e a_first a_last
+        b_link e_link a_link a_entry w0 w1 w2 w3 n1 n2
+        ba a_flag ea assertN EN φ :
     isCorrectPC_range pc_p pc_b pc_e a_first a_last →
     contiguous_between a a_first a_last →
     (* linking table assumptions *)
     withinBounds b_link e_link a_entry = true →
-    (a_link + f_a)%a = Some a_entry ->
+    (a_link + f_a)%a = Some a_entry →
+    ↑assertN ⊆ EN →
     (* condition for assertion success *)
-    (w_r = WInt z) ->
+    (n1 = n2) →
 
-    ▷ assert_r_z a f_a r z
+    ▷ assert a f_a
+    ∗ na_inv logrel_nais assertN (assert_inv ba a_flag ea)
+    ∗ na_own logrel_nais EN
     ∗ ▷ PC ↦ᵣ WCap pc_p pc_b pc_e a_first
     ∗ ▷ pc_b ↦ₐ WCap RO b_link e_link a_link
-    ∗ ▷ a_entry ↦ₐ fail_cap
-    ∗ ▷ r ↦ᵣ w_r
-    ∗ ▷ (∃ w, r_t1 ↦ᵣ w)
-    ∗ ▷ (∃ w, r_t2 ↦ᵣ w)
-    ∗ ▷ (∃ w, r_t3 ↦ᵣ w)
-    ∗ ▷ (r_t1 ↦ᵣ WInt 0%Z ∗ r_t2 ↦ᵣ WInt 0%Z ∗ r_t3 ↦ᵣ WInt 0%Z ∗ r ↦ᵣ WInt 0%Z
-         ∗ PC ↦ᵣ WCap pc_p pc_b pc_e a_last ∗ assert_r_z a f_a r z
-         ∗ pc_b ↦ₐ WCap RO b_link e_link a_link ∗ a_entry ↦ₐ fail_cap
+    ∗ ▷ a_entry ↦ₐ WCap E ba ea ba
+    ∗ ▷ r_t0 ↦ᵣ w0
+    ∗ ▷ r_t1 ↦ᵣ w1
+    ∗ ▷ r_t2 ↦ᵣ w2
+    ∗ ▷ r_t3 ↦ᵣ w3
+    ∗ ▷ r_t4 ↦ᵣ WInt n1
+    ∗ ▷ r_t5 ↦ᵣ WInt n2
+    ∗ ▷ (r_t0 ↦ᵣ w0 ∗
+         r_t1 ↦ᵣ WInt 0%Z ∗ r_t2 ↦ᵣ WInt 0%Z ∗ r_t3 ↦ᵣ WInt 0%Z
+         ∗ r_t4 ↦ᵣ WInt 0%Z ∗ r_t5 ↦ᵣ WInt 0%Z
+         ∗ PC ↦ᵣ WCap pc_p pc_b pc_e a_last ∗ assert a f_a
+         ∗ na_own logrel_nais EN
+         ∗ pc_b ↦ₐ WCap RO b_link e_link a_link ∗ a_entry ↦ₐ WCap E ba ea ba
          -∗ WP Seq (Instr Executable) {{ φ }})
     ⊢
     WP Seq (Instr Executable) {{ φ }}.
   Proof.
-    iIntros (Hvpc Hcont Hwb Htable Hsuccess)
-            "(>Hprog & >HPC & >Hpc_b & >Ha_entry & >Hr & >Hr_t1 & >Hr_t2 & >Hr_t3 & Hφ)".
+    iIntros (Hvpc Hcont Hwb Htable HN Hsuccess)
+            "(>Hprog & #Hinv & Hna & >HPC & >Hpc_b & >Ha_entry & >Hr_t0 & >Hr_t1 & >Hr_t2 & >Hr_t3 & >Hr_t4 & >Hr_t5 & Hφ)".
      (* fetch f *)
     iDestruct (contiguous_between_program_split with "Hprog") as (fetch_prog rest link)
                                                                    "(Hfetch & Hprog & #Hcont)";[apply Hcont|].
     iDestruct "Hcont" as %(Hcont_fetch & Hcont_rest & Heqapp & Hlink).
-    iDestruct "Hr_t1" as (w1) "Hr_t1".
-    iDestruct "Hr_t2" as (w2) "Hr_t2".
-    iDestruct "Hr_t3" as (w3) "Hr_t3".
-    iApply (fetch_spec with "[$HPC $Hfetch $Hr_t1 $Hr_t2 $Hr_t3 $Ha_entry $Hpc_b Hφ Hprog Hr]");
+    iApply (fetch_spec with "[- $HPC $Hfetch $Hr_t1 $Hr_t2 $Hr_t3 $Ha_entry $Hpc_b]");
       [|apply Hcont_fetch|apply Hwb|apply Htable|].
     { intros mid Hmid. apply isCorrectPC_inrange with a_first a_last; auto.
       apply contiguous_between_bounds in Hcont_rest. revert Hcont_rest Hmid; clear. solve_addr. }
@@ -229,166 +219,65 @@ Section macros.
     { intros mid Hmid. apply isCorrectPC_inrange with a_first a_last; auto. revert Hmid Hlink;clear. solve_addr. }
     destruct rest as [|a0 l'];[inversion Hlength_rest|].
     apply contiguous_between_cons_inv_first in Hcont_rest as Heq. subst a0.
-    (* sub_r_z r r z *)
-    destruct l';[inversion Hlength_rest|].
-    inversion Hsuccess. subst w_r.
+    (* move r_t2 r_t0 *)
+    destruct l';[inversion Hlength_rest|]. subst n2.
     iPrologue "Hprog".
-    iApply (wp_add_sub_lt_success_dst_z with "[$HPC $Hi $Hr]");
-      [apply decode_encode_instrW_inv|right;left;eauto|iContiguous_next Hcont_rest 0|iCorrectPC link a_last|..].
-    iEpilogue "(HPC & Hi & Hr)"; iCombine "Hfetch" "Hi" as "Hprog_done".
-    (* jnz r_t1 r *)
-    rewrite /= Z.sub_diag.
+    iApply (wp_move_success_reg with "[$HPC $Hi $Hr_t2 $Hr_t0]");
+      [apply decode_encode_instrW_inv|iCorrectPC link a_last|iContiguous_next Hcont_rest 0|].
+    iEpilogue "(HPC & Hi & Hr_t2 & Hr_t0)"; iCombine "Hfetch" "Hi" as "Hprog_done".
+    (* move r_t0 PC *)
     destruct l';[inversion Hlength_rest|].
     iPrologue "Hprog".
-    iApply (wp_jnz_success_next with "[$HPC $Hi $Hr_t1 $Hr]");
+    iApply (wp_move_success_reg_fromPC with "[$HPC $Hi $Hr_t0]");
       [apply decode_encode_instrW_inv|iCorrectPC link a_last|iContiguous_next Hcont_rest 1|].
-    iEpilogue "(HPC & Hinstr & Hr_t1 & Hr)". iCombine "Hinstr" "Hprog_done" as "Hprog_done".
+    iEpilogue "(HPC & Hi & Hr_t0)"; iCombine "Hi" "Hprog_done" as "Hprog_done".
+    (* lea r_t0 3 *)
+    destruct l';[inversion Hlength_rest|].
+    destruct l';[inversion Hlength_rest|].
+    iPrologue "Hprog".
+    assert (pc_p ≠ E).
+    { assert (isCorrectPC (WCap pc_p pc_b pc_e a_first)) as HH.
+      { apply Hvpc. split. solve_addr.
+        apply contiguous_between_length in Hcont.
+        rewrite Heqapp app_length /= in Hcont. solve_addr. }
+      destruct pc_p; inversion HH; destruct_or?; auto. }
+    iApply (wp_lea_success_z with "[$HPC $Hi $Hr_t0]");
+      [apply decode_encode_instrW_inv|iCorrectPC link a_last|..].
+    { iContiguous_next Hcont_rest 2. }
+    { eapply (contiguous_between_incr_addr_middle' _ _ _ 1%nat 3).
+      apply Hcont_rest. 2: done. 2: done. cbn. lia. } auto.
+    iEpilogue "(HPC & Hi & Hr_t0)"; iCombine "Hi" "Hprog_done" as "Hprog_done".
+    (* jmp r_t1 *)
+    iPrologue "Hprog".
+    iApply (wp_jmp_success with "[$HPC $Hi $Hr_t1]");
+      [apply decode_encode_instrW_inv|iCorrectPC link a_last|].
+    iEpilogue "(HPC & Hi & Hr_t1)"; iCombine "Hi" "Hprog_done" as "Hprog_done".
+    (* assert routine *)
+    iApply (assert_success_spec with "[- $Hinv $Hna $HPC $Hr_t0 $Hr_t4 $Hr_t5]"); auto.
+    iNext. iIntros "(Hna & HPC & Hr_t0 & Hr_t4 & Hr_t5)".
+    rewrite updatePcPerm_cap_non_E//.
+    (* move r_t0 r_t2 *)
+    destruct l';[inversion Hlength_rest|].
+    iPrologue "Hprog".
+    iApply (wp_move_success_reg with "[$HPC $Hi $Hr_t0 $Hr_t2]");
+      [apply decode_encode_instrW_inv|iCorrectPC link a_last|iContiguous_next Hcont_rest 4|].
+    iEpilogue "(HPC & Hi & Hr_t0 & Hr_t2)"; iCombine "Hi" "Hprog_done" as "Hprog_done".
     (* move r_t1 0 *)
-    destruct l';[|inversion Hlength_rest].
-    apply contiguous_between_last with (ai:=a1) in Hcont_rest as Hlink';[|auto].
+    destruct l';[inversion Hlength_rest|].
     iPrologue "Hprog".
     iApply (wp_move_success_z with "[$HPC $Hi $Hr_t1]");
-      [apply decode_encode_instrW_inv|iCorrectPC link a_last|apply Hlink'|auto|..].
+      [apply decode_encode_instrW_inv|iCorrectPC link a_last|iContiguous_next Hcont_rest 5|].
     iEpilogue "(HPC & Hi & Hr_t1)"; iCombine "Hi" "Hprog_done" as "Hprog_done".
+    (* move r_t2 0 *)
+    destruct l';[|inversion Hlength_rest].
+    apply contiguous_between_last with (ai:=a5) in Hcont_rest as Hlink';[|auto].
+    iPrologue "Hprog".
+    iApply (wp_move_success_z with "[$HPC $Hi $Hr_t2]");
+      [apply decode_encode_instrW_inv|iCorrectPC link a_last|apply Hlink'|auto|..].
+    iEpilogue "(HPC & Hi & Hr_t2)"; iCombine "Hi" "Hprog_done" as "Hprog_done".
     (* Continuation *)
     iApply "Hφ". iFrame.
-    rewrite Heqapp /=. iDestruct "Hprog_done" as "(?&?&?&?)". iFrame. done.
-  Qed.
-
-  (* Spec for assertion failure *)
-  (* When the assertion fails, the program jumps to the failure subroutine, sets the
-     flag (which by convention is one address after subroutine) and Fails *)
-  Lemma assert_r_z_fail a f_a r z pc_p pc_b pc_e a_first a_last z_r
-        b_link e_link a_link a_entry
-        f_b f_e f_a_first f_a_last a' a_env (* fail subroutine *)
-        flag_p flag_b flag_e flag_a (* flag capability *) :
-    isCorrectPC_range pc_p pc_b pc_e a_first a_last →
-    contiguous_between a a_first a_last →
-    (* linking table assumptions *)
-    withinBounds b_link e_link a_entry = true →
-    (a_link + f_a)%a = Some a_entry ->
-    (* failure subroutine assumptions *)
-    isCorrectPC_range RX f_b f_e f_a_first f_a_last →
-    contiguous_between a' f_a_first f_a_last →
-    (f_a_first + (length a'))%a = Some a_env ->
-    withinBounds f_b f_e a_env = true ->
-    (* flag assumptions *)
-    withinBounds flag_b flag_e flag_a = true ∧ writeAllowed flag_p = true ->
-    (* condition for assertion success *)
-    (z_r ≠ z) ->
-
-    (* the assert and assert failure subroutine programs *)
-    {{{ ▷ assert_r_z a f_a r z
-    ∗ ▷ assert_fail a'
-    ∗ ▷ PC ↦ᵣ WCap pc_p pc_b pc_e a_first
-    (* linking table and assertion flag *)
-    ∗ ▷ pc_b ↦ₐ WCap RO b_link e_link a_link (* the linking table capability *)
-    ∗ ▷ a_entry ↦ₐ WCap E f_b f_e f_a_first (* the capability to the failure subroutine *)
-    ∗ ▷ a_env ↦ₐ WCap flag_p flag_b flag_e flag_a (* the assertion flag capability *)
-    ∗ ▷ (∃ w, flag_a ↦ₐ w) (* the assertion flag *)
-    (* registers *)
-    ∗ ▷ r ↦ᵣ WInt z_r
-    ∗ ▷ (∃ w, r_t1 ↦ᵣ w)
-    ∗ ▷ (∃ w, r_t2 ↦ᵣ w)
-    ∗ ▷ (∃ w, r_t3 ↦ᵣ w) }}}
-
-      Seq (Instr Executable)
-
-    {{{ RET HaltedV; r_t1 ↦ᵣ WInt 0%Z ∗ r_t2 ↦ᵣ WInt 0%Z ∗ r_t3 ↦ᵣ WInt 0%Z ∗ (∃ z, r ↦ᵣ WInt z ∧ ⌜z ≠ 0⌝)
-         ∗ PC ↦ᵣ WCap RX f_b f_e (^(f_a_last + (-1))%a)
-         ∗ assert_r_z a f_a r z ∗ assert_fail a'
-         ∗ pc_b ↦ₐ WCap RO b_link e_link a_link ∗ a_entry ↦ₐ WCap E f_b f_e f_a_first
-         ∗ a_env ↦ₐ WCap flag_p flag_b flag_e flag_a ∗ flag_a ↦ₐ WInt 1%Z }}}.
-  Proof.
-    iIntros (Hvpc Hcont Hwb Htable Hvpc' Hcont' Henv Henvwb [Hwb' Hwa] Hfailure φ)
-            "(>Hprog & >Hprog' & >HPC & >Hpc_b & >Ha_entry & >Ha_env & >Hflag & >Hr & >Hr_t1 & >Hr_t2 & >Hr_t3) Hφ".
-    iDestruct "Hflag" as (flag_w) "Hflag".
-    (* fetch f *)
-    iDestruct (contiguous_between_program_split with "Hprog") as (fetch_prog rest link)
-                                                                   "(Hfetch & Hprog & #Hcont)";[apply Hcont|].
-    iDestruct "Hcont" as %(Hcont_fetch & Hcont_rest & Heqapp & Hlink).
-    iDestruct "Hr_t1" as (w1) "Hr_t1".
-    iDestruct "Hr_t2" as (w2) "Hr_t2".
-    iDestruct "Hr_t3" as (w3) "Hr_t3".
-    iApply (fetch_spec with "[$HPC $Hfetch $Hr_t1 $Hr_t2 $Hr_t3 $Ha_entry $Hpc_b Hφ Hprog Hr Hprog' Ha_env Hflag]");
-      [|apply Hcont_fetch|apply Hwb|apply Htable|].
-    { intros mid Hmid. apply isCorrectPC_inrange with a_first a_last; auto.
-      apply contiguous_between_bounds in Hcont_rest. revert Hcont_rest Hmid; clear. solve_addr. }
-    iNext. iIntros "(HPC & Hfetch& Hr_t1 & Hr_t2 & Hr_t3 & Hpc_b & Ha_entry)".
-    iDestruct (big_sepL2_length with "Hprog") as %Hlength_rest.
-    assert (isCorrectPC_range pc_p pc_b pc_e link a_last) as Hvpc_rest.
-    { intros mid Hmid. apply isCorrectPC_inrange with a_first a_last; auto. revert Hmid Hlink;clear. solve_addr. }
-    destruct rest as [|a0 l'];[inversion Hlength_rest|].
-    apply contiguous_between_cons_inv_first in Hcont_rest as Heq. subst a0.
-    (* sub_r_z r r z *)
-    destruct l';[inversion Hlength_rest|].
-    iPrologue "Hprog".
-    iApply (wp_add_sub_lt_success_dst_z with "[$HPC $Hi $Hr]");
-      [apply decode_encode_instrW_inv|right;left;eauto|iContiguous_next Hcont_rest 0|iCorrectPC link a_last|..].
-    iEpilogue "(HPC & Hi & Hr)"; iCombine "Hi" "Hfetch" as "Hprog_done".
-    (* jnz r_t1 r *)
-    iPrologue "Hprog".
-    iApply (wp_jnz_success_jmp with "[$HPC $Hi $Hr_t1 $Hr]");
-      [apply decode_encode_instrW_inv|iCorrectPC link a_last|simpl;revert Hfailure;clear;intros Hne Hcontr;simplify_eq;lia|..].
-    iEpilogue "(HPC & Hi & Hr_t1 & Hr)"; iSimpl in "HPC"; iCombine "Hi" "Hprog_done" as "Hprog_done".
-    iCombine "Hprog" "Hprog_done" as "Hprog_done".
-    (* FAILURE SUBROUTINE *)
-    iDestruct (big_sepL2_length with "Hprog'") as %Hlength'.
-    destruct a';[inversion Hlength'|].
-    apply contiguous_between_cons_inv_first in Hcont' as Heq. subst a1.
-    (* move r_t1 PC *)
-    destruct a';[inversion Hlength'|].
-    iAssert (⌜r_t1 ≠ PC⌝)%I as %Hne.
-    { iIntros (Hcontr). rewrite Hcontr. iDestruct (regname_dupl_false with "Hr_t1 HPC") as "H". done. }
-    iPrologue "Hprog'".
-    iApply (wp_move_success_reg_fromPC with "[$HPC $Hi $Hr_t1]");
-      [apply decode_encode_instrW_inv|iCorrectPC f_a_first f_a_last|iContiguous_next Hcont' 0|auto|..].
-    iEpilogue "(HPC & Hi & Hr_t1)". iRename "Hi" into "Hprog_done'".
-    (* lea r_t1 5 *)
-    destruct a';[inversion Hlength'|].
-    iPrologue "Hprog".
-    assert ((f_a_first + 6)%a = Some a_env) as Hlea.
-    { simpl in Henv. inversion Hlength' as [Heq]. rewrite Heq in Henv. auto. }
-    iApply (wp_lea_success_z with "[$HPC $Hi $Hr_t1]");
-      [apply decode_encode_instrW_inv|iCorrectPC f_a_first f_a_last|iContiguous_next Hcont' 1|apply Hlea|auto..].
-    iEpilogue "(HPC & Hi & Hr_t1)". iCombine "Hi" "Hprog_done'" as "Hprog_done'".
-    (* load r_t1 r_t1 *)
-    destruct a';[inversion Hlength'|].
-    iPrologue "Hprog".
-    iAssert (⌜(a_env =? a2)%a = false⌝)%I as %Hne'.
-    { destruct (decide (a_env = a2)%Z); [subst|iPureIntro;apply Z.eqb_neq,neq_z_of;auto].
-      iExFalso. iApply (addr_dupl_false with "Hi Ha_env"). }
-    iApply (wp_load_success_same with "[$HPC $Hi $Hr_t1 Ha_env]");
-      [|apply decode_encode_instrW_inv|iCorrectPC f_a_first f_a_last|auto|auto|iContiguous_next Hcont' 2|
-       rewrite Hne';iFrame|rewrite Hne'];auto. 
-    iEpilogue "(HPC & Hr_t1 & Hi & Ha_env)". iCombine "Hi" "Hprog_done" as "Hprog_done".
-    (* store r_t1 1 *)
-    destruct a';[inversion Hlength'|].
-    iPrologue "Hprog".
-    iApply (wp_store_success_z with "[$HPC $Hi $Hr_t1 $Hflag]");
-      [apply decode_encode_instrW_inv|iCorrectPC f_a_first f_a_last|iContiguous_next Hcont' 3|
-       auto|auto|].
-    iEpilogue "(HPC & Hi & Hr_t1 & Hflag)"; iCombine "Hi" "Hprog_done" as "Hprog_done".
-    (* move r_t1 0 *)
-    destruct a';[inversion Hlength'|].
-    iPrologue "Hprog".
-    iApply (wp_move_success_z with "[$HPC $Hi $Hr_t1]");
-      [apply decode_encode_instrW_inv|iCorrectPC f_a_first f_a_last|iContiguous_next Hcont' 4|].
-    iEpilogue "(HPC & Hi & Hr_t1)"; iCombine "Hi" "Hprog_done" as "Hprog_done".
-    (* Halt *)
-    destruct a';[|inversion Hlength'].
-    apply contiguous_between_last with (ai:=a5) in Hcont' as Hlink';[|auto].
-    iPrologue "Hprog".
-    iApply (wp_halt with "[$HPC $Hi]");
-      [apply decode_encode_instrW_inv|iCorrectPC f_a_first f_a_last|].
-    iEpilogue "(HPC & Hi)".
-    iApply wp_value. iApply "Hφ".
-    iFrame. iSplitL "Hr".
-    { simpl. iExists _. iFrame. iPureIntro. revert Hfailure. clear. lia. }
-    assert ((f_a_last + (-1))%a = Some a5) as ->;[|simpl].
-    { eapply contiguous_between_last in Hcont';[|eauto]. revert Hlink' Hcont'. clear. solve_addr. }
-    iFrame. rewrite Heqapp. iDestruct "Hprog_done'" as "(?&?)". iDestruct "Hprog_done" as "(?&?&?&?&?&?&?)".
-    iFrame.
+    rewrite Heqapp /=. iDestruct "Hprog_done" as "(?&?&?&?&?&?&?&?)". iFrame. done.
   Qed.
 
   (* --------------------------------------------------------------------------------- *)
